Translator and examples tweaked.

examples/miniML/ml_translatorLib.sig
@@ -18,5 +18,11 @@ sig
     val add_type_inv   : term -> unit
     val store_eval_thm : thm -> thm
     val store_eq_thm   : thm -> thm
+    val register_type  : hol_type -> unit
+
+    (* interface for producing output from translations *)
+
+    val clear_filename : unit -> unit
+    val set_filename   : string -> unit
 
 end
