examples/miniML/okasaki-examples/PairingHeapScript.sml
@@ -20,12 +20,12 @@ val pairing_heap_to_bag_def = Define `
   BAG_INSERT x (pairing_heaps_to_bag hs)) ∧
 
 (pairing_heaps_to_bag [] = {||}) ∧
-(pairing_heaps_to_bag (h::hs) = 
+(pairing_heaps_to_bag (h::hs) =
   BAG_UNION (pairing_heap_to_bag h) (pairing_heaps_to_bag hs))`;
 
 val pairing_heap_ok_def = tDefine "pairing_heap_ok" `
 (pairing_heap_ok get_key leq Empty = T) ∧
-(pairing_heap_ok get_key leq (Node x hs) = 
+(pairing_heap_ok get_key leq (Node x hs) =
   EVERY (pairing_heap_ok get_key leq) hs ∧
   BAG_EVERY (\y. leq (get_key x) (get_key y)) (pairing_heaps_to_bag hs))`
 (wf_rel_tac `measure (\(_,_,h). (heap_size (\x.1) h))` >>
@@ -48,7 +48,7 @@ val merge_def = Define `
 (merge get_key leq (Node x hs1) (Node y hs2) =
   if leq (get_key x) (get_key y) then
     Node x (Node y hs2 :: hs1)
-  else 
+  else
     Node y (Node x hs1 :: hs2))`;
 
 val merge_ind = fetch "-" "merge_ind"
@@ -59,7 +59,7 @@ insert get_key leq x h = merge get_key leq (Node x []) h`;
 val merge_pairs_def = Define `
 (merge_pairs get_key leq [] = Empty) ∧
 (merge_pairs get_key leq [h] = h) ∧
-(merge_pairs get_key leq (h1::h2::hs) = 
+(merge_pairs get_key leq (h1::h2::hs) =
   merge get_key leq (merge get_key leq h1 h2) (merge_pairs get_key leq hs))`;
 
 val merge_pairs_ind = fetch "-" "merge_pairs_ind"
@@ -72,17 +72,17 @@ delete_min get_key leq (Node x hs) = merge_pairs get_key leq hs`;
 
 val pairing_heap_merge_bag = Q.store_thm ("pairing_heap_merge_bag",
 `!get_key leq h1 h2.
-  pairing_heap_to_bag (merge get_key leq h1 h2) = 
+  pairing_heap_to_bag (merge get_key leq h1 h2) =
   BAG_UNION (pairing_heap_to_bag h1) (pairing_heap_to_bag h2)`,
 HO_MATCH_MP_TAC merge_ind >>
 srw_tac [BAG_AC_ss] [merge_def, pairing_heap_to_bag_def, BAG_INSERT_UNION]);
 
 val pairing_heap_merge_ok = Q.store_thm ("pairing_heap_merge_ok",
-`!get_key leq h1 h2. 
-  WeakLinearOrder leq ∧ 
-  pairing_heap_ok get_key leq h1 ∧ 
-  pairing_heap_ok get_key leq h2 
-  ⇒ 
+`!get_key leq h1 h2.
+  WeakLinearOrder leq ∧
+  pairing_heap_ok get_key leq h1 ∧
+  pairing_heap_ok get_key leq h2
+  ⇒
   pairing_heap_ok get_key leq (merge get_key leq h1 h2)`,
 HO_MATCH_MP_TAC merge_ind >>
 rw [merge_def, pairing_heap_ok_def, pairing_heap_to_bag_def] >>
@@ -97,19 +97,19 @@ rw [insert_def, pairing_heap_merge_bag, pairing_heap_to_bag_def,
     BAG_INSERT_UNION]);
 
 val pairing_heap_insert_ok = Q.store_thm ("pairing_heap_insert_ok",
-`!get_key leq x h. 
-  WeakLinearOrder leq ∧ pairing_heap_ok get_key leq h 
-  ⇒ 
+`!get_key leq x h.
+  WeakLinearOrder leq ∧ pairing_heap_ok get_key leq h
+  ⇒
   pairing_heap_ok get_key leq (insert get_key leq x h)`,
 rw [insert_def] >>
-`pairing_heap_ok get_key leq (Node x [])` 
+`pairing_heap_ok get_key leq (Node x [])`
          by rw [pairing_heap_ok_def, pairing_heap_to_bag_def] >>
 metis_tac [pairing_heap_merge_ok]);
 
 val pairing_heap_find_min_thm = Q.store_thm ("pairing_heap_find_min_thm",
 `!h get_key leq. WeakLinearOrder leq ∧ (h ≠ Empty) ∧ pairing_heap_ok get_key leq h ⇒
   BAG_IN (find_min h) (pairing_heap_to_bag h) ∧
-  (!y. BAG_IN y (pairing_heap_to_bag h) ⇒ 
+  (!y. BAG_IN y (pairing_heap_to_bag h) ⇒
        leq (get_key (find_min h)) (get_key y))`,
 rw [] >>
 cases_on `h` >>
@@ -126,19 +126,19 @@ srw_tac [BAG_ss]
 val pairing_heap_merge_pairs_ok = Q.prove (
 `!get_key leq hs.
   WeakLinearOrder leq ∧ EVERY (pairing_heap_ok get_key leq) hs
-  ⇒ 
+  ⇒
   pairing_heap_ok get_key leq (merge_pairs get_key leq hs)`,
 recInduct merge_pairs_ind >>
 rw [merge_pairs_def, pairing_heap_ok_def, pairing_heap_merge_ok]);
 
 val pairing_heap_delete_min_thm = Q.store_thm ("pairing_heap_delete_min_thm",
-`!h get_key leq. 
+`!h get_key leq.
   WeakLinearOrder leq ∧
-  (h ≠ Empty) ∧ 
-  pairing_heap_ok get_key leq h 
-  ⇒ 
+  (h ≠ Empty) ∧
+  pairing_heap_ok get_key leq h
+  ⇒
   pairing_heap_ok get_key leq (delete_min get_key leq h) ∧
-  (pairing_heap_to_bag (delete_min get_key leq h) = 
+  (pairing_heap_to_bag (delete_min get_key leq h) =
    BAG_DIFF (pairing_heap_to_bag h) (EL_BAG (find_min h)))`,
 rw [] >>
 cases_on `h` >>
@@ -146,12 +146,52 @@ fs [delete_min_def, pairing_heap_ok_def, pairing_heap_merge_pairs_bag] >-
 metis_tac [pairing_heap_merge_pairs_ok] >>
 rw [pairing_heap_to_bag_def, find_min_def, BAG_DIFF_INSERT2]);
 
-(* translator diverges
+
+
+val res = translate APPEND (* teaching the translator about lists... *)
+
+(* register heap -- begin *)
+
+(* val _ = register_type ``:'a heap`` *)
+
+val ty = ``:'a heap``
+
+val _ = delete_const "heap" handle _ => ()
+
+val tm =
+``(heap a Empty v ⇔ (v = Conv (SOME "EMPTY") []) ∧ T) ∧
+  (heap a (Node x2_1 x2_2) v ⇔
+   ∃v2_1 v2_2.
+     (v = Conv (SOME "NODE") [v2_1; v2_2]) ∧ a x2_1 v2_1 ∧
+     list (\x v. if MEM x x2_2 then heap a x v else ARB) x2_2 v2_2)``
+
+val inv_def = tDefine "heap_def" [ANTIQUOTE tm]
+ (WF_REL_TAC `measure (heap_size (\x.0) o FST o SND)`
+  \\ Induct
+  \\ EVAL_TAC \\ SIMP_TAC std_ss []
+  \\ REPEAT STRIP_TAC \\ RES_TAC
+  \\ FULL_SIMP_TAC std_ss [] \\ DECIDE_TAC)
+
+val list_SIMP = prove(
+  ``!xs b. list (\x v. if b x \/ MEM x xs then p x v else q) xs = list p xs``,
+  Induct
+  \\ FULL_SIMP_TAC std_ss [FUN_EQ_THM,fetch "-" "list_def",MEM,DISJ_ASSOC])
+  |> Q.SPECL [`xs`,`\x.F`] |> SIMP_RULE std_ss [];
+
+val inv_def = inv_def |> SIMP_RULE std_ss [list_SIMP]
+                      |> CONV_RULE (DEPTH_CONV ETA_CONV)
+
+val _ = set_inv_def (ty,inv_def)
+
+val _ = register_type ``:'a heap``
+
+(* register heap -- end *)
+
 val res = translate is_empty_def;
 val res = translate merge_def;
 val res = translate insert_def;
 val res = translate find_min_def;
+val res = translate merge_pairs_def;
 val res = translate delete_min_def;
-*)
 
 val _ = export_theory ()
