examples/miniML/okasaki-examples/ImplicitQueueScript.sml
@@ -1,0 +1,156 @@
+
+open HolKernel Parse boolLib bossLib; val _ = new_theory "ImplicitQueue";
+
+open listTheory arithmeticTheory;
+open ml_translatorLib;
+
+(* implementation *)
+
+val _ = Hol_datatype `times = Once of 'a | Twice of times => times`;
+val _ = Hol_datatype `digit = Zero | One of 'a times | Two of 'a times => 'a times`;
+val _ = Hol_datatype `queue = Shallow of 'a digit
+                            | Deep of 'a digit => queue => 'a digit`;
+
+val empty_def = Define `
+  empty = Shallow Zero`;
+
+val is_empty_def = Define `
+  (is_empty (Shallow Zero) = T) /\
+  (is_empty _ = F)`;
+
+val snoc_def = Define `
+  (snoc (Shallow Zero) y = Shallow (One y)) /\
+  (snoc (Shallow (One x)) y = Deep (Two x y) empty Zero) /\
+  (snoc (Deep f m Zero) y = Deep f m (One y)) /\
+  (snoc (Deep f m (One x)) y = Deep f (snoc m (Twice x y)) Zero)`
+
+val head_def = Define `
+  (head (Shallow (One x)) = x) /\
+  (head (Deep (One x) m r) = x) /\
+  (head (Deep (Two x y) m r) = x)`;
+
+val tail_def = Define `
+  (tail (Shallow (One x)) = empty) /\
+  (tail (Deep (Two x y) m r) = Deep (One y) m r) /\
+  (tail (Deep (One x) q r) =
+     if is_empty q then Shallow r else
+       case head q of Twice y z => Deep (Two y z) (tail q) r)`
+
+
+(* translation *)
+
+val _ = set_filename (current_theory())
+
+val res = translate empty_def
+val res = translate is_empty_def
+val res = translate snoc_def
+val res = translate head_def
+val res = translate tail_def
+
+(*
+(* verification *)
+
+val exps_def = Define `
+  (exps (Once x) = [x]) /\
+  (exps (Twice t1 t2) = exps t1 ++ exps t2)`;
+
+val digits_def = Define `
+  (digits Zero = []) /\
+  (digits (One x) = exps x) /\
+  (digits (Two x y) = exps x ++ exps y)`;
+
+val flatten_def = Define `
+  (flatten (Shallow x) = digits x) /\
+  (flatten (Deep d1 t d2) = digits d1 ++ flatten t ++ digits d2)`;
+
+val only_digits_def = Define `
+  (only_digits Zero = []) /\
+  (only_digits (One x) = [x]) /\
+  (only_digits (Two x y) = [x;y])`;
+
+val depth_def = Define `
+  (depth n m (Once x) = (m = n)) /\
+  (depth n m (Twice t1 t2) = depth (n+1) m t1 /\ depth (n+1) m t2)`;
+
+val ddepth_def = Define `
+  ddepth n d = EVERY (\d. depth 0 n d) (only_digits d)`;
+
+val two_def = Define `
+  (two (Two _ _) = T) /\ (two _ = F)`;
+
+val queue_ok_def = Define `
+  (queue_ok n (Shallow x) = ~two x /\ ddepth n x) /\
+  (queue_ok n (Deep x1 t x2) =
+     ~(x1 = Zero) /\ queue_ok (n+1) t /\ ~two x2 /\ ddepth n x1 /\ ddepth n x2)`;
+
+val queue_inv_def = Define `
+  queue_inv q t = queue_ok 0 t /\ (q = flatten t)`;
+
+val empty_thm = prove(
+  ``queue_inv [] empty``,
+  EVAL_TAC);
+
+val exps_NOT_NIL = prove(
+  ``!e. ~(exps e = [])``,
+  Induct THEN EVAL_TAC THEN FULL_SIMP_TAC std_ss [APPEND_eq_NIL]);
+
+val is_empty_thm = prove(
+  ``!xs q. queue_inv xs q ==> (is_empty q = (xs = []))``,
+  Cases THEN Cases THEN EVAL_TAC
+  THEN1 (Cases_on `d` THEN EVAL_TAC THEN SIMP_TAC std_ss [exps_NOT_NIL])
+  THEN1 (Cases_on `d0` THEN EVAL_TAC THEN ONCE_REWRITE_TAC [EQ_SYM_EQ]
+         THEN SIMP_TAC std_ss [exps_NOT_NIL,APPEND_eq_NIL])
+  THEN Cases_on `d` THEN EVAL_TAC);
+
+val qdepth_def = Define `
+  (qdepth (Shallow _) = 0) /\
+  (qdepth (Deep _ t _) = SUC (qdepth t))`;
+
+val snoc_thm = prove(
+  ``!q xs x. queue_inv xs q ==> queue_inv (xs ++ [x]) (snoc q (Once x))``,
+  STRIP_TAC THEN SIMP_TAC std_ss [queue_inv_def] THEN Q.SPEC_TAC (`0`,`n`)
+  THEN Induct_on `qdepth q` THEN STRIP_TAC THEN STRIP_TAC
+
+snoc_def
+
+queue_ok_def
+
+  Cases_on `q` THEN EVAL_TAC
+  THEN Cases_on `d` THEN EVAL_TAC THEN FULL_SIMP_TAC (srw_ss()) []
+
+
+val depth_LESS_EQ = prove(
+  ``!e m n. depth m n e ==> m <= n``,
+  Induct THEN EVAL_TAC THEN REPEAT STRIP_TAC THEN RES_TAC THEN DECIDE_TAC);
+
+val depth_00 = prove(
+  ``!e. depth 0 0 e ==> ?x. e = Once x``,
+  Cases THEN SIMP_TAC (srw_ss()) [depth_def] THEN REPEAT STRIP_TAC
+  THEN METIS_TAC [depth_LESS_EQ,EVAL ``1 <= 0:num``]);
+
+val head_thm = prove(
+  ``!q x xs. queue_inv (x::xs) q ==> (head q = Once x)``,
+  Cases THEN TRY (Cases_on `d`) THEN TRY (Cases_on `d0`)
+  THEN EVAL_TAC THEN SIMP_TAC (srw_ss()) []
+  THEN REPEAT STRIP_TAC THEN IMP_RES_TAC depth_00
+  THEN FULL_SIMP_TAC (srw_ss()) [exps_def])
+
+val tail_thm = prove(
+  ``!q x xs. queue_inv (x::xs) q ==> queue_inv xs (tail q)``,
+  Cases THEN1 (Cases_on `d` THEN EVAL_TAC THEN SIMP_TAC (srw_ss()) []
+    THEN REPEAT STRIP_TAC THEN IMP_RES_TAC depth_00
+    THEN FULL_SIMP_TAC (srw_ss()) [exps_def])
+  THEN REVERSE (Cases_on `d0`) THEN EVAL_TAC THEN SIMP_TAC (srw_ss()) []
+  THEN1 (REPEAT STRIP_TAC THEN IMP_RES_TAC depth_00
+         THEN FULL_SIMP_TAC (srw_ss()) [exps_def])
+  THEN Cases_on `is_empty q'` THEN FULL_SIMP_TAC (srw_ss()) []
+  THEN1
+   (Cases_on `q'` THEN FULL_SIMP_TAC std_ss [is_empty_def]
+    THEN Cases_on `d'` THEN FULL_SIMP_TAC std_ss [is_empty_def]
+    THEN EVAL_TAC THEN FULL_SIMP_TAC std_ss [is_empty_def]
+    THEN REPEAT STRIP_TAC THEN IMP_RES_TAC depth_00
+    THEN FULL_SIMP_TAC (srw_ss()) [exps_def])
+
+*)
+
+val _ = export_theory();
