examples/miniML/okasaki-examples/LeftistHeapScript.sml
@@ -1,5 +1,6 @@
 open bossLib Theory Parse boolTheory pairTheory Defn Tactic boolLib bagTheory
-open relationTheory bagLib miscTheory lcsymtacs ml_translatorLib;
+open relationTheory bagLib miscTheory lcsymtacs;
+open ml_translatorLib;
 
 val fs = full_simp_tac (srw_ss ())
 val rw = srw_tac []
@@ -143,13 +144,14 @@ fs [delete_min_def, leftist_heap_ok_def, leftist_heap_merge_bag] >-
 metis_tac [leftist_heap_merge_ok] >>
 rw [leftist_heap_to_bag_def, find_min_def, BAG_DIFF_INSERT2]);
 
+
 val res = translate is_empty_def;
 val res = translate rank_def;
-(* Type inference failure 
 val res = translate make_node_def;
+val res = translate APPEND;
 val res = translate merge_def;
 val res = translate insert_def;
 val res = translate find_min_def;
 val res = translate delete_min_def;
-*)
+
 val _ = export_theory ();
